Updated permission lattice, more work on the expression relation and related lemmas

case_study/MinimalCaps/Model.v
@@ -385,17 +385,19 @@ Module MinCapsModel.
         + apply submseteq_cons; trivial.
     Qed.
 
-    Lemma safe_sub_range (b' e' b e : Addr) :
-      forall p a,
+    (* TODO: should be possible to get rid of this once the Model and ghost stmts etc
+             are updated sufficiently. *)
+    Lemma safe_sub_range (b' e' b e a a' : Addr) :
+      forall p,
         ⊢ ⌜ (b <= b')%Z /\ (e' <= e)%Z ⌝ -∗
                                             interp
                                             (inr {| cap_permission := p; cap_begin := b; cap_end := e; cap_cursor := a |}) -∗
                                                                                                                               interp
-                                                                                                                              (inr {| cap_permission := p; cap_begin := b'; cap_end := e'; cap_cursor := a |}).
+                                                                                                                              (inr {| cap_permission := p; cap_begin := b'; cap_end := e'; cap_cursor := a' |}).
     Proof.
-      iIntros (p a) "/= [% %] Hsafe".
+      iIntros (p) "/= [% %] Hsafe".
       do 2 rewrite fixpoint_interp1_eq.
-      destruct p; try (by iFrame); simpl; try iDestruct "Hsafe" as "/= [Hsafe | %]";
+      induction p; try (by iFrame); try iDestruct "Hsafe" as "/= [Hsafe | %]";
         try (iRight; iPureIntro; lia).
       - iLeft.
         iIntros "%".
@@ -454,6 +456,192 @@ Module MinCapsModel.
     Global Instance interp_Persistent (w : leibnizO MemVal) : Persistent (interp w).
     Proof. destruct w; simpl; rewrite fixpoint_interp1_eq; simpl; first apply _.
            destruct c; destruct cap_permission; apply _. Qed.
+
+    Definition IH : iProp Σ :=
+      (□ ▷ (∀ p b e a,
+               interp_gprs interp
+            -∗ reg_pointsTo pc (MkCap p b e a)
+            -∗ □ interp (inr (MkCap p b e a)) -∗ interp_loop (sg := SailGS _ _ mG))).
+
+    Lemma interp_subperm_weaken p p' b e a :
+      p' ≠ E ->
+      Subperm p' p ->
+      interp (inr (MkCap p b e a)) -∗
+      interp (inr (MkCap p' b e a)).
+    Proof.
+      intros HpnotE Hp; destruct p'; destruct p; inversion Hp; auto; iIntros "H";
+        rewrite !fixpoint_interp1_eq; try done.
+    Qed.
+
+    (* TODO: a lot of repetition, pull it into separate lemma and apply it *)
+    Lemma interp_weakening p p' b b' e e' a a' :
+      p ≠ E ->
+      (b ≤ b')%Z ->
+      (e' ≤ e)%Z ->
+      Subperm p' p ->
+      IH -∗
+      interp (inr (MkCap p b e a)) -∗
+      interp (inr (MkCap p' b' e' a')).
+    Proof.
+      intros HpnotE Hb He Hsubperm.
+      iIntros "#IH #HA".
+      destruct (decide (b' ≤ e')%Z).
+      2: {
+        rewrite !fixpoint_interp1_eq.
+        destruct p; try done;
+        destruct p'; try done;
+        try (iRight; auto;
+             iPureIntro;
+             apply Znot_le_gt in n;
+               by apply Z.gt_lt in n).
+        do 2 iModIntro.
+        iIntros "(Hpc & Hreg0 & Hreg1 & Hreg2 & Hreg3 & _)".
+        iApply ("IH" with "[-Hpc IH HA] Hpc"); try iFrame.
+        done.
+        iModIntro.
+        rewrite fixpoint_interp1_eq; simpl.
+        iRight;
+          iPureIntro;
+          apply Znot_le_gt in n;
+          by apply Z.gt_lt in n.
+        do 2 iModIntro.
+        iIntros "(Hpc & Hreg0 & Hreg1 & Hreg2 & Hreg3 & _)".
+        iApply ("IH" with "[-Hpc IH HA] Hpc"); try iFrame.
+        done.
+        iModIntro.
+        rewrite fixpoint_interp1_eq; simpl.
+        iRight;
+          iPureIntro;
+          apply Znot_le_gt in n;
+          by apply Z.gt_lt in n.
+      }
+      destruct p'.
+      - rewrite !fixpoint_interp1_eq; done.
+      - destruct p; inversion Hsubperm.
+        + rewrite !fixpoint_interp1_eq; simpl.
+          iLeft.
+          iIntros (_).
+          iDestruct "HA" as "[HA | %]"; try lia.
+          assert (Hle : (b ≤ e)%Z).
+          { eapply Z.le_trans. apply Hb.
+            eapply Z.le_trans. apply l. apply He. }
+          iSpecialize ("HA" $! Hle).
+          iDestruct "HA" as "([%Hbl %Hel] & HA)".
+          iSplitR.
+          iPureIntro.
+          split;
+            (eapply le_liveAddrs;
+             first apply (conj Hbl Hel));
+            intuition;
+            try assumption.
+          eapply Z.le_trans; first apply l; auto.
+          eapply Z.le_trans; first apply Hb; auto.
+          iApply (region_addrs_submseteq $! (conj Hb He) with "HA").
+        + rewrite !fixpoint_interp1_eq; simpl.
+          iLeft.
+          iIntros (_).
+          iDestruct "HA" as "[HA | %]"; try lia.
+          assert (Hle : (b ≤ e)%Z).
+          { eapply Z.le_trans. apply Hb.
+            eapply Z.le_trans. apply l. apply He. }
+          iSpecialize ("HA" $! Hle).
+          iDestruct "HA" as "([%Hbl %Hel] & HA)".
+          iSplitR.
+          iPureIntro.
+          split;
+            (eapply le_liveAddrs;
+             first apply (conj Hbl Hel));
+            intuition;
+            try assumption.
+          eapply Z.le_trans; first apply l; auto.
+          eapply Z.le_trans; first apply Hb; auto.
+          iApply (region_addrs_submseteq $! (conj Hb He) with "HA").
+      - destruct p; inversion Hsubperm.
+        + rewrite !fixpoint_interp1_eq; simpl.
+          iLeft.
+          iIntros (_).
+          iDestruct "HA" as "[HA | %]"; try lia.
+          assert (Hle : (b ≤ e)%Z).
+          { eapply Z.le_trans. apply Hb.
+            eapply Z.le_trans. apply l. apply He. }
+          iSpecialize ("HA" $! Hle).
+          iDestruct "HA" as "([%Hbl %Hel] & HA)".
+          iSplitR.
+          iPureIntro.
+          split;
+            (eapply le_liveAddrs;
+             first apply (conj Hbl Hel));
+            intuition;
+            try assumption.
+          eapply Z.le_trans; first apply l; auto.
+          eapply Z.le_trans; first apply Hb; auto.
+          iApply (region_addrs_submseteq $! (conj Hb He) with "HA").
+      - destruct p; inversion Hsubperm.
+        + rewrite !fixpoint_interp1_eq.
+          do 2 iModIntro.
+          iIntros "(Hpc & Hreg0 & Hreg1 & Hreg2 & Hreg3 & _)".
+          iApply ("IH" with "[-Hpc IH HA] Hpc"); try iFrame.
+          done.
+          iModIntro.
+          rewrite !fixpoint_interp1_eq; simpl.
+          iLeft.
+          iIntros (_).
+          iDestruct "HA" as "[HA | %]"; try lia.
+          assert (Hle : (b ≤ e)%Z).
+          { eapply Z.le_trans. apply Hb.
+            eapply Z.le_trans. apply l. apply He. }
+          iSpecialize ("HA" $! Hle).
+          iDestruct "HA" as "([%Hbl %Hel] & HA)".
+          iSplitR.
+          iPureIntro.
+          split;
+            (eapply le_liveAddrs;
+             first apply (conj Hbl Hel));
+            intuition;
+            try assumption.
+          eapply Z.le_trans; first apply l; auto.
+          eapply Z.le_trans; first apply Hb; auto.
+          iApply (region_addrs_submseteq $! (conj Hb He) with "HA").
+        + rewrite !fixpoint_interp1_eq.
+          do 2 iModIntro.
+          iIntros "(Hpc & Hreg0 & Hreg1 & Hreg2 & Hreg3 & _)".
+          iApply ("IH" with "[-Hpc IH HA] Hpc"); try iFrame.
+          done.
+          iModIntro.
+          rewrite !fixpoint_interp1_eq; simpl.
+          iLeft.
+          iIntros (_).
+          iDestruct "HA" as "[HA | %]"; try lia.
+          assert (Hle : (b ≤ e)%Z).
+          { eapply Z.le_trans. apply Hb.
+            eapply Z.le_trans. apply l. apply He. }
+          iSpecialize ("HA" $! Hle).
+          iDestruct "HA" as "([%Hbl %Hel] & HA)".
+          iSplitR.
+          iPureIntro.
+          split;
+            (eapply le_liveAddrs;
+             first apply (conj Hbl Hel));
+            intuition;
+            try assumption.
+          eapply Z.le_trans; first apply l; auto.
+          eapply Z.le_trans; first apply Hb; auto.
+          iApply (region_addrs_submseteq $! (conj Hb He) with "HA").
+        + contradiction.
+    Qed.
+
+    Lemma subseg_interp_preserved p b b' e e' a a' :
+      p ≠ E ->
+      (b ≤ b')%Z ->
+      (e' ≤ e)%Z ->
+      IH -∗
+      interp (inr (MkCap p b e a)) -∗
+      interp (inr (MkCap p b' e' a')).
+    Proof.
+      iIntros (HpnotE Hb He) "#IH Hinterp".
+      iApply (interp_weakening with "IH Hinterp"); auto.
+      destruct p; reflexivity.
+    Qed.
   End Predicates.
 
   Module MinCapsIrisPredicates <: IrisPredicates MinCapsBase MinCapsSignature MinCapsSemantics MinCapsIrisPrelims MinCapsIrisParams MinCapsIrisResources.
@@ -498,6 +686,7 @@ Module MinCapsModel2.
   Import MinCapsSignature.
   Import MinCapsSpecification.
   Import MinCapsProgram.
+  Import MinCapsIrisPrelims.
   Import MinCapsIrisParams.
   Import MinCapsIrisResources.
   Module Import MinCapsIrisModel := IrisInstanceWithContracts MinCapsBase MinCapsSignature MinCapsSpecification MinCapsSemantics MinCapsIrisPrelims MinCapsIrisParams MinCapsIrisResources MinCapsIrisPredicates MinCapsModel MinCapsModel.
